ironfleet/src/Dafny/Distributed/Concur/Refinement.i.dfy
@@ -9,17 +9,50 @@ module RefinementModule {
     type SpecState
     predicate SpecInit(ss:SpecState)
     predicate SpecNext(ss:SpecState, ss':SpecState)
-    predicate SpecCorrespondence(ds:DistributedSystem, ss:SpecState)
+    predicate SpecCorrespondence(ds:DistributedSystemState, ss:SpecState)
 
-    lemma {:axiom} lemma_RightMoverForwardPreservation(rightMover:Entry, ds:DistributedSystem, ds':DistributedSystem, ss:SpecState)
+    lemma {:axiom} lemma_RightMoverForwardPreservation(rightMover:Entry, ds:DistributedSystemState, ds':DistributedSystemState, ss:SpecState)
         requires DistributedSystemNextEntryAction(ds, ds', rightMover);
         requires SpecCorrespondence(ds, ss);
         ensures  SpecCorrespondence(ds', ss);
 
-    lemma {:axiom} lemma_LeftMoverBackwardPreservation(leftMover:Entry, ds:DistributedSystem, ds':DistributedSystem, ss:SpecState)
+    lemma {:axiom} lemma_LeftMoverBackwardPreservation(leftMover:Entry, ds:DistributedSystemState, ds':DistributedSystemState, ss:SpecState)
         requires DistributedSystemNextEntryAction(ds, ds', leftMover);
         requires SpecCorrespondence(ds', ss);
         ensures  SpecCorrespondence(ds, ss);
+
+    predicate IsValidSpecBehavior(sb:seq<SpecState>)
+    {
+           |sb| > 0
+        && SpecInit(sb[0])
+        && (forall i :: 0 <= i < |sb| - 1 ==> (SpecNext(sb[i], sb[i+1]) || sb[i] == sb[i+1]))
+    }
+
+    predicate IsValidDistributedSystemBehavior(db:seq<DistributedSystemState>)
+    {
+           |db| > 0
+        && DistributedSystemInit(db[0])
+        && (forall i :: 0 <= i < |db| - 1 ==> DistributedSystemNext(db[i], db[i+1]))
+    }
+
+    predicate IsValidDistributedSystemTraceAndBehavior(trace:Trace, db:seq<DistributedSystemState>)
+    {
+           |db| == |trace| + 1
+        && DistributedSystemInit(db[0])
+        && (forall i :: 0 <= i < |db| - 1 ==> DistributedSystemNextEntryAction(db[i], db[i+1], trace[i]))
+    }
+
+    predicate DistributedSystemBehaviorRefinesSpecBehavior(db:seq<DistributedSystemState>, sb:seq<SpecState>)
+    {
+           |db| == |sb|
+        && IsValidSpecBehavior(sb)
+        && (forall i :: 0 <= i < |db| ==> SpecCorrespondence(db[i], sb[i]))
+    }
+
+    predicate DistributedSystemBehaviorRefinesSpec(db:seq<DistributedSystemState>)
+    {
+        exists sb :: DistributedSystemBehaviorRefinesSpecBehavior(db, sb)
+    }
 
 }
 
